pulse/ulib/experimental/Steel.SpinLock.fsti
@@ -2,13 +2,13 @@ module Steel.SpinLock
 open Steel.Effect
 open Steel.Memory
 
-val lock (p:hprop) : Type u#0
+val lock (p:hprop u#1) : Type u#0
 
-val new_lock (p:hprop)
+val new_lock (p:hprop u#1)
   : SteelT (lock p) p (fun _ -> emp)
 
-val acquire (#p:hprop) (l:lock p)
+val acquire (#p:hprop u#1) (l:lock p)
   : SteelT unit emp (fun _ -> p)
 
-val release (#p:hprop) (l:lock p)
+val release (#p:hprop u#1) (l:lock p)
   : SteelT unit p (fun _ -> emp)
